add circuit transforms

cava/Cava/Lib/CircuitTransforms.v
@@ -14,13 +14,11 @@
 (* limitations under the License.                                           *)
 (****************************************************************************)
 
-Require Export Cava.Lib.Lib.
-Require Export Cava.Lib.AddersProperties.
-Require Export Cava.Lib.CavaPreludeProperties.
-Require Export Cava.Lib.CircuitTransformsProperties.
-Require Export Cava.Lib.CombinationalProperties.
-Require Export Cava.Lib.CombinatorsProperties.
-Require Export Cava.Lib.DecoderProperties.
-Require Export Cava.Lib.MultiplexersProperties.
-Require Export Cava.Lib.MultipliersProperties.
-Require Export Cava.Lib.VecProperties.
+Require Import Cava.Core.Core.
+
+Section WithCava.
+  Context `{semantics : Cava}.
+
+  (* identity circuit *)
+  Definition Id {t} : Circuit t t := Comb Monad.ret.
+End WithCava.
