cava/Cava/Lib/CircuitTransformsProperties.v
@@ -1,0 +1,115 @@
+(****************************************************************************)
+(* Copyright 2021 The Project Oak Authors                                   *)
+(*                                                                          *)
+(* Licensed under the Apache License, Version 2.0 (the "License")           *)
+(* you may not use this file except in compliance with the License.         *)
+(* You may obtain a copy of the License at                                  *)
+(*                                                                          *)
+(*     http://www.apache.org/licenses/LICENSE-2.0                           *)
+(*                                                                          *)
+(* Unless required by applicable law or agreed to in writing, software      *)
+(* distributed under the License is distributed on an "AS IS" BASIS,        *)
+(* WITHOUT WARRANTIES OR CONDITIONS OF ANY KIND, either express or implied. *)
+(* See the License for the specific language governing permissions and      *)
+(* limitations under the License.                                           *)
+(****************************************************************************)
+
+Require Import Coq.Classes.Morphisms.
+Require Import coqutil.Tactics.Tactics.
+Require Import Cava.Core.Core.
+Require Import Cava.Semantics.Combinational.
+Require Import Cava.Semantics.Equivalence.
+Require Import Cava.Lib.CircuitTransforms.
+Require Import Cava.Util.Tactics.
+Import Circuit.Notations.
+
+Local Ltac simplify :=
+  cbn [circuit_state step Id]; intros;
+  destruct_products; cbn [fst snd] in *;
+  repeat (destruct_pair_let; cbn [fst snd]);
+  logical_simplify; simpl_ident; subst.
+
+Lemma First_Id t1 t2 : @cequiv (t1 * t2) (t1 * t2) (First Id) Id.
+Proof.
+  exists eq. ssplit; [ reflexivity | ]. simplify. ssplit; reflexivity.
+Qed.
+Hint Rewrite @First_Id using solve [eauto] : circuitsimpl.
+
+Lemma Second_Id t1 t2 : @cequiv (t1 * t2) (t1 * t2) (Second Id) Id.
+Proof.
+  exists eq. ssplit; [ reflexivity | ]. simplify. ssplit; reflexivity.
+Qed.
+Hint Rewrite @Second_Id using solve [eauto] : circuitsimpl.
+
+Lemma Compose_Id_l i o c : @cequiv i o (Id >==> c) c.
+Proof.
+  exists (fun (st1 : unit * circuit_state c) (st2 : circuit_state c) => st1 = (tt, st2)).
+  ssplit; [ reflexivity | ]. simplify. ssplit; reflexivity.
+Qed.
+Hint Rewrite @Compose_Id_l using solve [eauto] : circuitsimpl.
+
+Lemma Compose_Id_r i o c : @cequiv i o (c >==> Id) c.
+Proof.
+  exists (fun (st1 : circuit_state c * unit) (st2 : circuit_state c) => st1 = (st2, tt)).
+  ssplit; [ reflexivity | ]. simplify. ssplit; reflexivity.
+Qed.
+Hint Rewrite @Compose_Id_r using solve [eauto] : circuitsimpl.
+
+Lemma Compose_assoc A B C D
+      (f : Circuit A B) (g : Circuit B C) (h : Circuit C D) :
+  cequiv (f >==> (g >==> h)) (f >==> g >==> h).
+Proof.
+  exists (fun (st1 : circuit_state f * (circuit_state g * circuit_state h))
+       (st2 : circuit_state f * circuit_state g * circuit_state h) =>
+       st1 = (fst (fst st2), (snd (fst st2), snd st2))).
+  ssplit; [ reflexivity | ]. simplify. ssplit; reflexivity.
+Qed.
+
+Lemma First_Compose A B C D (f : Circuit A B) (g : Circuit B C) :
+  @cequiv (A * D) (C * D) (First (f >==> g)) (First f >==> First g).
+Proof.
+  exists eq. ssplit; [ reflexivity | ]. simplify. ssplit; reflexivity.
+Qed.
+Hint Rewrite @First_Compose using solve [eauto] : circuitsimpl.
+
+Lemma Second_Compose A B C D (f : Circuit A B) (g : Circuit B C) :
+  @cequiv (D * A) (D * C) (Second (f >==> g)) (Second f >==> Second g).
+Proof.
+  exists eq. ssplit; [ reflexivity | ]. simplify. ssplit; reflexivity.
+Qed.
+Hint Rewrite @Second_Compose using solve [eauto] : circuitsimpl.
+
+Lemma LoopInitCE_First_r A B C s reset
+      (body : Circuit (A * combType s) (B * combType s))
+      (f : Circuit B C) :
+  cequiv (LoopInitCE reset (body >==> First f)) (LoopInitCE reset body >==> f).
+Proof.
+  exists (fun (st1 : circuit_state body * circuit_state f * combType s)
+       (st2 : circuit_state body * combType s * circuit_state f) =>
+       st1 = (fst (fst st2), snd st2, snd (fst st2))).
+  ssplit; [ reflexivity | ]. simplify. ssplit; reflexivity.
+Qed.
+Hint Rewrite @LoopInitCE_First_r using solve [eauto] : push_loop.
+
+Lemma LoopInit_First_r A B C s reset
+      (body : Circuit (A * combType s) (B * combType s))
+      (f : Circuit B C) :
+  cequiv (LoopInit reset (body >==> First f)) (LoopInit reset body >==> f).
+Proof.
+  cbv [LoopInit]. simpl_ident. rewrite <-Compose_assoc, LoopInitCE_First_r. reflexivity.
+Qed.
+Hint Rewrite @LoopInit_First_r using solve [eauto] : push_loop.
+
+Lemma LoopCE_First_r A B C s
+      (body : Circuit (A * combType s) (B * combType s))
+      (f : Circuit B C) :
+  cequiv (LoopCE (body >==> First f)) (LoopCE body >==> f).
+Proof. apply LoopInitCE_First_r. Qed.
+Hint Rewrite @LoopCE_First_r using solve [eauto] : push_loop.
+
+Lemma Loop_First_r A B C s
+      (body : Circuit (A * combType s) (B * combType s))
+      (f : Circuit B C) :
+  cequiv (Loop (body >==> First f)) (Loop body >==> f).
+Proof. apply LoopInit_First_r. Qed.
+Hint Rewrite @Loop_First_r using solve [eauto] : push_loop.
